pulse/src/ocaml/plugin/generated/Pulse_Checker_Auto_IntroRewrite.ml
@@ -1,8 +1,7 @@
 open Prims
 let (intro_rewrite : Pulse_Checker_Auto_Util.intro_from_unmatched_fn) =
   fun g ->
-    fun ctxt ->
-      fun p ->
-        Obj.magic
-          (FStar_Tactics_Effect.lift_div_tac
-             (fun uu___ -> FStar_Pervasives_Native.None))
+    fun p ->
+      Obj.magic
+        (FStar_Tactics_Effect.lift_div_tac
+           (fun uu___ -> FStar_Pervasives_Native.None))
