pulse/src/ocaml/plugin/generated/Pulse_Checker_Auto_Prover.ml
@@ -51,7 +51,7 @@ let (init_prover_state :
         Pulse_Syntax_Base.st_term ->
           Pulse_Syntax_Base.comp_st ->
             (unit, unit, unit) Pulse_Typing.st_typing ->
-              (unit, unit) Pulse_Checker_Auto_Util.prover_state)
+              unit Pulse_Checker_Auto_Util.prover_state)
   =
   fun g ->
     fun ctxt ->
@@ -60,10 +60,14 @@ let (init_prover_state :
           fun c ->
             fun t_typing ->
               {
-                Pulse_Checker_Auto_Util.ctxt_typing = ();
-                Pulse_Checker_Auto_Util.t = t;
-                Pulse_Checker_Auto_Util.c = c;
-                Pulse_Checker_Auto_Util.t_typing = t_typing;
+                Pulse_Checker_Auto_Util.preamble =
+                  {
+                    Pulse_Checker_Auto_Util.ctxt = ctxt;
+                    Pulse_Checker_Auto_Util.ctxt_typing = ();
+                    Pulse_Checker_Auto_Util.t = t;
+                    Pulse_Checker_Auto_Util.c = c;
+                    Pulse_Checker_Auto_Util.t_typing = t_typing
+                  };
                 Pulse_Checker_Auto_Util.matched_pre =
                   Pulse_Syntax_Base.Tm_Emp;
                 Pulse_Checker_Auto_Util.unmatched_pre =
@@ -78,81 +82,57 @@ let (init_prover_state :
                      (proof_steps_idem_typing g ctxt));
                 Pulse_Checker_Auto_Util.pre_equiv = ()
               }
-let (step_intro_exists :
-  Pulse_Typing.env ->
-    Pulse_Syntax_Base.vprop ->
-      (unit, unit) Pulse_Checker_Auto_Util.prover_state ->
-        ((unit, unit) Pulse_Checker_Auto_Util.prover_state
-           FStar_Pervasives_Native.option,
-          unit) FStar_Tactics_Effect.tac_repr)
-  =
+let (step_intro_exists : Pulse_Checker_Auto_Util.prover_step_t) =
   fun g ->
-    fun o ->
-      fun p ->
-        FStar_Tactics_Effect.tac_bind
-          (FStar_Range.mk_range "Pulse.Checker.Auto.Prover.fst"
-             (Prims.of_int (54)) (Prims.of_int (4)) (Prims.of_int (54))
-             (Prims.of_int (51)))
-          (FStar_Range.mk_range "Pulse.Checker.Auto.Prover.fst"
-             (Prims.of_int (53)) (Prims.of_int (2)) (Prims.of_int (54))
-             (Prims.of_int (51)))
-          (Obj.magic (Pulse_Checker_Auto_IntroExists.intro_exists g o p))
-          (fun uu___ ->
-             (fun uu___ ->
-                Obj.magic
-                  (FStar_Tactics_Util.map_opt
-                     (Pulse_Checker_Auto_Util.apply_intro_from_unmatched_step
-                        g o p) uu___)) uu___)
-let (step_intro_pure :
-  Pulse_Typing.env ->
-    Pulse_Syntax_Base.vprop ->
-      (unit, unit) Pulse_Checker_Auto_Util.prover_state ->
-        ((unit, unit) Pulse_Checker_Auto_Util.prover_state
-           FStar_Pervasives_Native.option,
-          unit) FStar_Tactics_Effect.tac_repr)
-  =
+    fun p ->
+      FStar_Tactics_Effect.tac_bind
+        (FStar_Range.mk_range "Pulse.Checker.Auto.Prover.fst"
+           (Prims.of_int (56)) (Prims.of_int (4)) (Prims.of_int (56))
+           (Prims.of_int (51)))
+        (FStar_Range.mk_range "Pulse.Checker.Auto.Prover.fst"
+           (Prims.of_int (55)) (Prims.of_int (2)) (Prims.of_int (56))
+           (Prims.of_int (51)))
+        (Obj.magic (Pulse_Checker_Auto_IntroExists.intro_exists g p))
+        (fun uu___ ->
+           (fun uu___ ->
+              Obj.magic
+                (FStar_Tactics_Util.map_opt
+                   (Pulse_Checker_Auto_Util.apply_intro_from_unmatched_step g
+                      p) uu___)) uu___)
+let (step_intro_pure : Pulse_Checker_Auto_Util.prover_step_t) =
   fun g ->
-    fun o ->
-      fun p ->
-        FStar_Tactics_Effect.tac_bind
-          (FStar_Range.mk_range "Pulse.Checker.Auto.Prover.fst"
-             (Prims.of_int (60)) (Prims.of_int (4)) (Prims.of_int (60))
-             (Prims.of_int (47)))
-          (FStar_Range.mk_range "Pulse.Checker.Auto.Prover.fst"
-             (Prims.of_int (59)) (Prims.of_int (2)) (Prims.of_int (60))
-             (Prims.of_int (47)))
-          (Obj.magic (Pulse_Checker_Auto_IntroPure.intro_pure g o p))
-          (fun uu___ ->
-             (fun uu___ ->
-                Obj.magic
-                  (FStar_Tactics_Util.map_opt
-                     (Pulse_Checker_Auto_Util.apply_intro_from_unmatched_step
-                        g o p) uu___)) uu___)
-let (step_intro_rewrite :
-  Pulse_Typing.env ->
-    Pulse_Syntax_Base.vprop ->
-      (unit, unit) Pulse_Checker_Auto_Util.prover_state ->
-        ((unit, unit) Pulse_Checker_Auto_Util.prover_state
-           FStar_Pervasives_Native.option,
-          unit) FStar_Tactics_Effect.tac_repr)
-  =
+    fun p ->
+      FStar_Tactics_Effect.tac_bind
+        (FStar_Range.mk_range "Pulse.Checker.Auto.Prover.fst"
+           (Prims.of_int (61)) (Prims.of_int (4)) (Prims.of_int (61))
+           (Prims.of_int (47)))
+        (FStar_Range.mk_range "Pulse.Checker.Auto.Prover.fst"
+           (Prims.of_int (60)) (Prims.of_int (2)) (Prims.of_int (61))
+           (Prims.of_int (47)))
+        (Obj.magic (Pulse_Checker_Auto_IntroPure.intro_pure g p))
+        (fun uu___ ->
+           (fun uu___ ->
+              Obj.magic
+                (FStar_Tactics_Util.map_opt
+                   (Pulse_Checker_Auto_Util.apply_intro_from_unmatched_step g
+                      p) uu___)) uu___)
+let (step_intro_rewrite : Pulse_Checker_Auto_Util.prover_step_t) =
   fun g ->
-    fun o ->
-      fun p ->
-        FStar_Tactics_Effect.tac_bind
-          (FStar_Range.mk_range "Pulse.Checker.Auto.Prover.fst"
-             (Prims.of_int (66)) (Prims.of_int (4)) (Prims.of_int (66))
-             (Prims.of_int (53)))
-          (FStar_Range.mk_range "Pulse.Checker.Auto.Prover.fst"
-             (Prims.of_int (65)) (Prims.of_int (2)) (Prims.of_int (66))
-             (Prims.of_int (53)))
-          (Obj.magic (Pulse_Checker_Auto_IntroRewrite.intro_rewrite g o p))
-          (fun uu___ ->
-             (fun uu___ ->
-                Obj.magic
-                  (FStar_Tactics_Util.map_opt
-                     (Pulse_Checker_Auto_Util.apply_intro_from_unmatched_step
-                        g o p) uu___)) uu___)
+    fun p ->
+      FStar_Tactics_Effect.tac_bind
+        (FStar_Range.mk_range "Pulse.Checker.Auto.Prover.fst"
+           (Prims.of_int (66)) (Prims.of_int (4)) (Prims.of_int (66))
+           (Prims.of_int (53)))
+        (FStar_Range.mk_range "Pulse.Checker.Auto.Prover.fst"
+           (Prims.of_int (65)) (Prims.of_int (2)) (Prims.of_int (66))
+           (Prims.of_int (53)))
+        (Obj.magic (Pulse_Checker_Auto_IntroRewrite.intro_rewrite g p))
+        (fun uu___ ->
+           (fun uu___ ->
+              Obj.magic
+                (FStar_Tactics_Util.map_opt
+                   (Pulse_Checker_Auto_Util.apply_intro_from_unmatched_step g
+                      p) uu___)) uu___)
 let rec (first_success :
   Pulse_Checker_Auto_Util.prover_step_t Prims.list ->
     Pulse_Checker_Auto_Util.prover_step_t)
@@ -160,40 +140,36 @@ let rec (first_success :
   fun uu___ ->
     (fun l ->
        fun g ->
-         fun o ->
-           fun p ->
-             match l with
-             | [] ->
-                 Obj.magic
-                   (Obj.repr
-                      (FStar_Tactics_Effect.lift_div_tac
-                         (fun uu___ -> FStar_Pervasives_Native.None)))
-             | s::l1 ->
-                 Obj.magic
-                   (Obj.repr
-                      (FStar_Tactics_Effect.tac_bind
-                         (FStar_Range.mk_range
-                            "Pulse.Checker.Auto.Prover.fst"
-                            (Prims.of_int (73)) (Prims.of_int (12))
-                            (Prims.of_int (73)) (Prims.of_int (15)))
-                         (FStar_Range.mk_range
-                            "Pulse.Checker.Auto.Prover.fst"
-                            (Prims.of_int (73)) (Prims.of_int (6))
-                            (Prims.of_int (75)) (Prims.of_int (24)))
-                         (Obj.magic (s g o p))
-                         (fun uu___ ->
-                            (fun uu___ ->
-                               match uu___ with
-                               | FStar_Pervasives_Native.None ->
-                                   Obj.magic
-                                     (Obj.repr (first_success l1 g o p))
-                               | FStar_Pervasives_Native.Some p1 ->
-                                   Obj.magic
-                                     (Obj.repr
-                                        (FStar_Tactics_Effect.lift_div_tac
-                                           (fun uu___1 ->
-                                              FStar_Pervasives_Native.Some p1))))
-                              uu___)))) uu___
+         fun p ->
+           match l with
+           | [] ->
+               Obj.magic
+                 (Obj.repr
+                    (FStar_Tactics_Effect.lift_div_tac
+                       (fun uu___ -> FStar_Pervasives_Native.None)))
+           | s::l1 ->
+               Obj.magic
+                 (Obj.repr
+                    (FStar_Tactics_Effect.tac_bind
+                       (FStar_Range.mk_range "Pulse.Checker.Auto.Prover.fst"
+                          (Prims.of_int (73)) (Prims.of_int (12))
+                          (Prims.of_int (73)) (Prims.of_int (15)))
+                       (FStar_Range.mk_range "Pulse.Checker.Auto.Prover.fst"
+                          (Prims.of_int (73)) (Prims.of_int (6))
+                          (Prims.of_int (75)) (Prims.of_int (24)))
+                       (Obj.magic (s g p))
+                       (fun uu___ ->
+                          (fun uu___ ->
+                             match uu___ with
+                             | FStar_Pervasives_Native.None ->
+                                 Obj.magic (Obj.repr (first_success l1 g p))
+                             | FStar_Pervasives_Native.Some p1 ->
+                                 Obj.magic
+                                   (Obj.repr
+                                      (FStar_Tactics_Effect.lift_div_tac
+                                         (fun uu___1 ->
+                                            FStar_Pervasives_Native.Some p1))))
+                            uu___)))) uu___
 let (step : Pulse_Checker_Auto_Util.prover_step_t) =
   first_success
     [Pulse_Checker_Auto_Framing.step_match;
@@ -202,91 +178,90 @@ let (step : Pulse_Checker_Auto_Util.prover_step_t) =
     step_intro_rewrite]
 let (finish :
   Pulse_Typing.env ->
-    Pulse_Syntax_Base.vprop ->
-      (unit, unit) Pulse_Checker_Auto_Util.prover_state ->
-        (Pulse_Syntax_Base.st_term, Pulse_Syntax_Base.comp_st,
-          (unit, unit, unit) Pulse_Typing.st_typing) FStar_Pervasives.dtuple3)
+    unit Pulse_Checker_Auto_Util.prover_state ->
+      (Pulse_Syntax_Base.st_term, Pulse_Syntax_Base.comp_st,
+        (unit, unit, unit) Pulse_Typing.st_typing) FStar_Pervasives.dtuple3)
   =
   fun g ->
-    fun o ->
-      fun p ->
-        let t_typing =
-          Pulse_Typing_Metatheory.st_typing_equiv_pre g
-            (Pulse_Checker_Auto_Util.__proj__Mkprover_state__item__t g o p)
-            (Pulse_Checker_Auto_Util.__proj__Mkprover_state__item__c g o p)
-            p.Pulse_Checker_Auto_Util.t_typing
-            p.Pulse_Checker_Auto_Util.matched_pre () in
-        let framing_token =
-          FStar_Pervasives.Mkdtuple3
-            ((Pulse_Checker_VPropEquiv.list_as_vprop
-                p.Pulse_Checker_Auto_Util.remaining_ctxt), (), ()) in
-        let uu___ =
-          Pulse_Checker_Framing.apply_frame g p.Pulse_Checker_Auto_Util.t
-            (Pulse_Checker_Auto_Util.proof_steps_post g o p) ()
-            (Pulse_Typing_Metatheory.comp_st_with_pre
-               p.Pulse_Checker_Auto_Util.c
-               p.Pulse_Checker_Auto_Util.matched_pre) t_typing framing_token in
-        match uu___ with
-        | Prims.Mkdtuple2 (uu___1, t_typing1) ->
-            let uu___2 =
-              Pulse_Checker_Auto_Util.bind_proof_steps_with g o p
-                p.Pulse_Checker_Auto_Util.t uu___1 t_typing1 in
-            (match uu___2 with
-             | Prims.Mkdtuple2 (t, t_typing2) ->
-                 FStar_Pervasives.Mkdtuple3
-                   (t, (Pulse_Typing_Metatheory.comp_st_with_pre uu___1 o),
-                     t_typing2))
+    fun p ->
+      let t_typing =
+        Pulse_Typing_Metatheory.st_typing_equiv_pre g
+          (Pulse_Checker_Auto_Util.__proj__Mkprover_state_preamble__item__t g
+             p.Pulse_Checker_Auto_Util.preamble)
+          (Pulse_Checker_Auto_Util.__proj__Mkprover_state_preamble__item__c g
+             p.Pulse_Checker_Auto_Util.preamble)
+          (p.Pulse_Checker_Auto_Util.preamble).Pulse_Checker_Auto_Util.t_typing
+          p.Pulse_Checker_Auto_Util.matched_pre () in
+      let framing_token =
+        FStar_Pervasives.Mkdtuple3
+          ((Pulse_Checker_VPropEquiv.list_as_vprop
+              p.Pulse_Checker_Auto_Util.remaining_ctxt), (), ()) in
+      let uu___ =
+        Pulse_Checker_Framing.apply_frame g
+          (p.Pulse_Checker_Auto_Util.preamble).Pulse_Checker_Auto_Util.t
+          (Pulse_Checker_Auto_Util.proof_steps_post g p) ()
+          (Pulse_Typing_Metatheory.comp_st_with_pre
+             (p.Pulse_Checker_Auto_Util.preamble).Pulse_Checker_Auto_Util.c
+             p.Pulse_Checker_Auto_Util.matched_pre) t_typing framing_token in
+      match uu___ with
+      | Prims.Mkdtuple2 (uu___1, t_typing1) ->
+          let uu___2 =
+            Pulse_Checker_Auto_Util.bind_proof_steps_with g p
+              (p.Pulse_Checker_Auto_Util.preamble).Pulse_Checker_Auto_Util.t
+              uu___1 t_typing1 in
+          (match uu___2 with
+           | Prims.Mkdtuple2 (t, t_typing2) ->
+               FStar_Pervasives.Mkdtuple3
+                 (t,
+                   (Pulse_Typing_Metatheory.comp_st_with_pre uu___1
+                      (p.Pulse_Checker_Auto_Util.preamble).Pulse_Checker_Auto_Util.ctxt),
+                   t_typing2))
 let (as_failure :
   Pulse_Typing.env ->
-    Pulse_Syntax_Base.vprop ->
-      (unit, unit) Pulse_Checker_Auto_Util.prover_state -> framing_failure)
+    unit Pulse_Checker_Auto_Util.prover_state -> framing_failure)
   =
   fun g ->
-    fun o ->
-      fun p ->
-        {
-          unmatched_preconditions = (p.Pulse_Checker_Auto_Util.unmatched_pre);
-          remaining_context = (p.Pulse_Checker_Auto_Util.remaining_ctxt)
-        }
+    fun p ->
+      {
+        unmatched_preconditions = (p.Pulse_Checker_Auto_Util.unmatched_pre);
+        remaining_context = (p.Pulse_Checker_Auto_Util.remaining_ctxt)
+      }
 let rec (solve :
   Pulse_Typing.env ->
-    Pulse_Syntax_Base.vprop ->
-      (unit, unit) Pulse_Checker_Auto_Util.prover_state ->
-        (((Pulse_Syntax_Base.st_term, Pulse_Syntax_Base.comp_st,
-            (unit, unit, unit) Pulse_Typing.st_typing)
-            FStar_Pervasives.dtuple3,
-           framing_failure) FStar_Pervasives.either,
-          unit) FStar_Tactics_Effect.tac_repr)
+    unit Pulse_Checker_Auto_Util.prover_state ->
+      (((Pulse_Syntax_Base.st_term, Pulse_Syntax_Base.comp_st,
+          (unit, unit, unit) Pulse_Typing.st_typing) FStar_Pervasives.dtuple3,
+         framing_failure) FStar_Pervasives.either,
+        unit) FStar_Tactics_Effect.tac_repr)
   =
   fun g ->
-    fun o ->
-      fun p ->
-        FStar_Tactics_Effect.tac_bind
-          (FStar_Range.mk_range "Pulse.Checker.Auto.Prover.fst"
-             (Prims.of_int (113)) (Prims.of_int (10)) (Prims.of_int (113))
-             (Prims.of_int (16)))
-          (FStar_Range.mk_range "Pulse.Checker.Auto.Prover.fst"
-             (Prims.of_int (113)) (Prims.of_int (4)) (Prims.of_int (118))
-             (Prims.of_int (20))) (Obj.magic (step g o p))
-          (fun uu___ ->
-             (fun uu___ ->
-                match uu___ with
-                | FStar_Pervasives_Native.None ->
-                    Obj.magic
-                      (Obj.repr
-                         (FStar_Tactics_Effect.lift_div_tac
-                            (fun uu___1 ->
-                               FStar_Pervasives.Inr (as_failure g o p))))
-                | FStar_Pervasives_Native.Some p1 ->
-                    Obj.magic
-                      (Obj.repr
-                         (match p1.Pulse_Checker_Auto_Util.unmatched_pre with
-                          | [] ->
-                              Obj.repr
-                                (FStar_Tactics_Effect.lift_div_tac
-                                   (fun uu___1 ->
-                                      FStar_Pervasives.Inl (finish g o p1)))
-                          | uu___1 -> Obj.repr (solve g o p1)))) uu___)
+    fun p ->
+      FStar_Tactics_Effect.tac_bind
+        (FStar_Range.mk_range "Pulse.Checker.Auto.Prover.fst"
+           (Prims.of_int (115)) (Prims.of_int (10)) (Prims.of_int (115))
+           (Prims.of_int (16)))
+        (FStar_Range.mk_range "Pulse.Checker.Auto.Prover.fst"
+           (Prims.of_int (115)) (Prims.of_int (4)) (Prims.of_int (120))
+           (Prims.of_int (20))) (Obj.magic (step g p))
+        (fun uu___ ->
+           (fun uu___ ->
+              match uu___ with
+              | FStar_Pervasives_Native.None ->
+                  Obj.magic
+                    (Obj.repr
+                       (FStar_Tactics_Effect.lift_div_tac
+                          (fun uu___1 ->
+                             FStar_Pervasives.Inr (as_failure g p))))
+              | FStar_Pervasives_Native.Some p1 ->
+                  Obj.magic
+                    (Obj.repr
+                       (match p1.Pulse_Checker_Auto_Util.unmatched_pre with
+                        | [] ->
+                            Obj.repr
+                              (FStar_Tactics_Effect.lift_div_tac
+                                 (fun uu___1 ->
+                                    FStar_Pervasives.Inl (finish g p1)))
+                        | uu___1 -> Obj.repr (solve g p1)))) uu___)
 let (prove_precondition :
   Pulse_Typing.env ->
     Pulse_Syntax_Base.term ->
@@ -306,4 +281,4 @@ let (prove_precondition :
         fun t ->
           fun c ->
             fun t_typing ->
-              solve g ctxt (init_prover_state g ctxt () t c t_typing)
+              solve g (init_prover_state g ctxt () t c t_typing)
