pulse/lib/steel/pulse/Pulse.Checker.Auto.IntroRewrite.fst
@@ -16,5 +16,5 @@ open Pulse.Typing
 module Metatheory = Pulse.Typing.Metatheory
 
 let intro_rewrite =
-  fun #g #ctxt p ->
+  fun #g p ->
   None
